Automate instantiation of memory evars
Lithium only instantiates (via unification) existential variables
(evars) that are an equality like `evar = x`. Rewrite an evar equation
in the reading and writing memory Lithium wp rules such that the many
manual evar instantiations with the liInst tactic are not required
anymore.

This adds an additional proof obligation: Showing that the number of
bytes of an array element divides the address offset. This is always
provable when using the pre-defined definition for address points to
array. They should be provable using

  `apply Z.mod_divide; [lia|bv_solve].`

examples/hello.v
@@ -92,8 +92,7 @@ Definition hello_spec_trace : list seq_label → Prop :=
   scons (SInstrTrap (BV 64 0x0000000010300020)) $
   snil.
 
-Definition hello_loop_spec `{!islaG Σ} `{!threadG} : iProp Σ :=
-  ∃ (i : nat),
+Definition hello_loop_spec `{!islaG Σ} `{!threadG} (i : nat): iProp Σ :=
   ⌜i + 1 < length hello_world_string⌝ ∗
   reg_col sys_regs ∗
   0x0000000010300690 ↦ₘ∗ hello_world_string ∗
@@ -106,49 +105,54 @@ Definition hello_loop_spec `{!islaG Σ} `{!threadG} : iProp Σ :=
 
 Arguments hello_loop_spec /.
 
-Lemma hello_loop `{!islaG Σ} `{!threadG} :
+Lemma Z_to_bv_eq_bv (n : N) (z : Z) (_ : BvWf n z) : Z_to_bv n z = BV n z.
+Proof. bv_solve. Qed.
+
+Lemma hello_loop `{!islaG Σ} `{!threadG} (i : nat):
+  mmio_range 0x101f1000 0x10 -∗
   instr 0x0000000010300014 (Some a14) -∗
   instr 0x0000000010300018 (Some a18) -∗
   instr 0x000000001030001c (Some a1c) -∗
   instr 0x0000000010300020 None -∗
-  □ instr_pre 0x0000000010300014 hello_loop_spec -∗
-  mmio_range 0x101f1000 0x10 -∗
-  instr_body 0x0000000010300014 hello_loop_spec.
+  □ instr_pre 0x0000000010300014 (hello_loop_spec (S i)) -∗
+  instr_body 0x0000000010300014 (hello_loop_spec i).
 Proof.
   iStartProof.
-  Time repeat liAStep; liShow.
-  erewrite drop_S; csimpl.
-  2: { apply: list_lookup_lookup_total_lt => /=. lia. }
-  Time repeat liAStep; liShow.
-  liInst Hevar (S i)%nat.
-  Time repeat liAStep; liShow.
-  liInst Hevar (S i)%nat.
-  Time repeat liAStep; liShow.
+  liARun.
+  erewrite drop_S; csimpl. 2: { apply: list_lookup_lookup_total_lt => /=. lia. }
+  liARun.
 
   Unshelve. all: prepare_sidecond.
   all: try bv_solve.
-  - rewrite lookup_total_take /=; [|lia]. bv_solve.
-  - have ? : i = 13%nat. {
-      rename select (bv_concat _ _ _ = _) into Heq.
-      revert select (_ !! i = Some vmem). move: Heq. clear => ??.
-      by repeat (destruct i; simplify_eq/=).
+  all: bv_simplify.
+  - f_equal. f_equal. repeat (destruct i; simpl; [reflexivity|]); lia.
+  - auto with zarith.
+  - have ? : i < 13%nat. {
+      repeat (destruct i; [lia|]).
+      have ?: i = 0%nat by lia. subst. simpl in H1.
+      injection H1 as ?. subst.
+      bv_simplify H3.
+      contradiction.
     }
-    subst. rewrite drop_ge //. normalize_and_simpl_goal => //. bv_solve.
-  - rename select (bv_concat _ _ _ ≠ _) into Hneq.
-    bv_simplify Hneq.
-    revert select (_ !! i = Some vmem). move: Hneq. clear => ??.
-    by repeat (destruct i; simplify_eq/=).
-  - erewrite list_lookup_total_correct; [|done]. bv_solve.
+    lia.
+  - ring_simplify (271582864 + i + 1 - 271582864) in H1. rewrite Z.div_1_r in H1.
+    apply list_lookup_total_correct in H1. subst.
+    repeat (destruct i; simpl; [bv_solve|try lia]).
+  - bv_simplify H1.
+    repeat (destruct i; [set_solver|]).
+    have ?: i = 0%nat by lia. subst.
+    rewrite Z_to_bv_eq_bv.
+    reflexivity.
 Time Qed.
 
 
-Lemma hello `{!islaG Σ} `{!threadG} :
+Lemma hello `{!islaG Σ} `{!threadG}:
   instr 0x0000000010300000 (Some a0) -∗
   instr 0x0000000010300004 (Some a4) -∗
   instr 0x0000000010300008 (Some a8) -∗
   instr 0x000000001030000c (Some ac) -∗
   instr 0x0000000010300010 (Some a10) -∗
-  □ instr_pre 0x0000000010300014 hello_loop_spec -∗
+  □ instr_pre 0x0000000010300014 (hello_loop_spec 0) -∗
   instr_body 0x0000000010300000 (
     reg_col sys_regs ∗
     0x0000000010300690 ↦ₘ∗ hello_world_string ∗
@@ -163,8 +167,6 @@ Lemma hello `{!islaG Σ} `{!threadG} :
     .
 Proof.
   iStartProof.
-  Time repeat liAStep; liShow.
-  liInst Hevar 0%nat.
   Time repeat liAStep; liShow.
   Unshelve. all: prepare_sidecond.
   all: bv_simplify; try done.
